lakefile.lean
@@ -12,3 +12,9 @@ lean_lib «Climber» where
 
 lean_exe «smoke» where
   root := `Smoke
+
+lean_exe «bedrock-smoke» where
+  root := `BedrockSmoke
+
+lean_exe «runner» where
+  root := `RunnerMain
